formal/AExp.thy
@@ -73,6 +73,9 @@ lemma aval_plus_symmetry: "aval (Plus x y) s = aval (Plus y x) s"
 abbreviation null_state ("<>") where
   "null_state \<equiv> (K$ None)"
 
+lemma default_empty: "infinite (UNIV :: 'a set) \<Longrightarrow> finfun_default (<>::'a \<Rightarrow>f 'b option) = None"
+  by (simp add: finfun_default_def finfun_default_aux_def)
+
 nonterminal maplets and maplet
 
 (* TODO: get the <1 := L (Num x)> kind of syntax back *)
