formal/inference/EFSM_Dot.thy
@@ -123,7 +123,7 @@ definition iefsm2dot :: "iEFSM \<Rightarrow> String.literal" where
                  STR ''  node [color=''+quote+(STR ''black'')+quote+STR '', fillcolor=''+quote+(STR ''white'')+quote+STR '', shape=''+quote+(STR ''circle'')+quote+STR '', style=''+quote+(STR ''filled'')+quote+STR '', fontname=''+quote+STR ''Latin Modern Math''+quote+STR ''];''+newline+
                  STR ''  edge [fontname=''+quote+STR ''Latin Modern Math''+quote+STR ''];''+newline+newline+
                   (join (map (\<lambda>s. STR ''  s''+show_nat s+STR ''[label=<s<sub>'' +show_nat s+ STR ''</sub>>];'') (sorted_list_of_fset (S e - {|0|}))) (newline))+newline+newline+
-                  (join ((map (\<lambda>(uid, (from, to), t). STR ''  s''+(show_nat from)+STR ''->s''+(show_nat to)+STR ''[label=<<i> (''+show_nat uid+STR '')''+(transition2dot t)+STR ''</i>>];'') (sorted_list_of_fset e))) newline)+newline+
+                  (join ((map (\<lambda>(uid, (from, to), t). STR ''  s''+(show_nat from)+STR ''->s''+(show_nat to)+STR ''[label=<<i> (''+show_nat uid+STR '')''+(transition2dot t)+STR ''</i>>];'') (sorted_list_of_fset (to_old_representation e)))) newline)+newline+
                 STR ''}''"
 
 abbreviation newline_str :: string where
@@ -137,6 +137,6 @@ definition iefsm2dot_str :: "iEFSM \<Rightarrow> string" where
                  ''  graph [rankdir=''@quote_str@''LR''@quote_str@'', fontname=''@quote_str@''Latin Modern Math''@quote_str@''];''@newline_str@
                  ''  node [color=''@quote_str@''black''@quote_str@'', fillcolor=''@quote_str@''white''@quote_str@'', shape=''@quote_str@''circle''@quote_str@'', style=''@quote_str@''filled''@quote_str@'', fontname=''@quote_str@''Latin Modern Math''@quote_str@''];''@newline_str@
                  ''  edge [fontname=''@quote_str@''Latin Modern Math''@quote_str@''];''@newline_str@
-                  (String.explode (join (sorted_list_of_fset (fimage (\<lambda>(uid, (from, to), t).STR ''  ''+(show_nat from)+STR ''->''+(show_nat to)+STR ''[label=<(''+(show_nat uid)+STR '') ''+(transition2dot t)+STR ''>]'') e)) newline)@newline_str)@
+                  (String.explode (join (sorted_list_of_fset (fimage (\<lambda>(uid, (from, to), t).STR ''  ''+(show_nat from)+STR ''->''+(show_nat to)+STR ''[label=<(''+(show_nat uid)+STR '') ''+(transition2dot t)+STR ''>]'') (to_old_representation e))) newline)@newline_str)@
                 ''}''"
 end
