formal/inference/heuristics/Ignore_Inputs.thy
@@ -3,7 +3,7 @@ imports "../Inference"
 begin
 
 definition enumerate_outputs :: "iEFSM \<Rightarrow> label \<Rightarrow> arity \<Rightarrow>  aexp list fset" where
-  "enumerate_outputs e l a = (fimage (\<lambda>(_, _, t). Outputs t) (ffilter (\<lambda>(_, _, t). Label t = l \<and> Arity t = a) e))"
+  "enumerate_outputs e l a = (fimage (\<lambda>(_, _, t). Outputs t) (ffilter (\<lambda>(_, _, t). Label t = l \<and> Arity t = a) (to_old_representation e)))"
 
 definition drop_guards :: "transition \<Rightarrow> transition" where
   "drop_guards t = \<lparr>Label = Label t, Arity = Arity t, Guard = [], Outputs = Outputs t, Updates = Updates t\<rparr>"
@@ -16,11 +16,11 @@ definition drop_inputs :: "update_modifier" where
      t1 = (get_by_id new t1ID);
      t2 = (get_by_id new t2ID) in
      if fis_singleton (enumerate_outputs new (Label t1) (Arity t1)) then
-     Some (fimage 
+     Some (to_new_representation (fimage 
       (\<lambda>(id, route, t). 
        if id = t1ID then
          (id, route, drop_guards t)
-       else (id, route, t)) (ffilter (\<lambda>(id, _). id \<noteq> t2ID) new))
+       else (id, route, t)) (ffilter (\<lambda>(id, _). id \<noteq> t2ID) (to_old_representation new))))
      else None
    )"
 
@@ -29,16 +29,7 @@ definition transitionwise_drop_inputs :: update_modifier where
      t1 = (get_by_id new t1ID);
      t2 = (get_by_id new t2ID) in
      if Outputs t1 = Outputs t2 then
-       Some (replace (drop_transition new t2ID) t1ID (drop_guards t1))
-     else
-       None)"
-
-definition statewise_drop_inputs :: "update_modifier" where
-  "statewise_drop_inputs t1ID t2ID s new old np = (let
-     t1 = (get_by_id new t1ID);
-     t2 = (get_by_id new t2ID) in
-     if \<forall>(_, t, _) |\<in>| outgoing_transitions s new. (Label t = Label t1 \<and> Arity t = Arity t1) \<longrightarrow> Outputs t = Outputs t1 then
-       Some (replace (drop_transitions new ((fimage (comp snd snd) (outgoing_transitions s new)) - {|t1ID|})) t1ID (drop_guards t1))
+       Some (replace_transitions new [(t1ID, origin t1ID new, dest t1ID new, (drop_guards t1)), (t2ID, origin t2ID new, dest t2ID new, (drop_guards t1))])
      else
        None)"
 
