formal/inference/heuristics/Least_Upper_Bound.thy
@@ -45,8 +45,8 @@ fun lob :: update_modifier where
      t2 = (get_by_id new t2ID) in
      case lob_aux t1 t2 of
        None \<Rightarrow> None |
-       Some lob_t \<Rightarrow> 
-      Some (replace (drop_transitions new {|t2ID|}) t1ID lob_t)
+       Some lob_t \<Rightarrow>
+           Some (replace_transitions new [(t1ID, origin t1ID new, dest t1ID new, lob_t), (t2ID, origin t2ID new, dest t2ID new, lob_t)])
    )"
 
 fun has_corresponding :: "gexp \<Rightarrow> gexp list \<Rightarrow> bool" where
@@ -614,7 +614,7 @@ fun gob :: update_modifier where
      case gob_aux t1 t2 of
        None \<Rightarrow> None |
        Some gob_t \<Rightarrow> 
-      Some (replace (drop_transitions new {|t2ID|}) t1ID gob_t)
+           Some (replace_transitions new [(t1ID, origin t1ID new, dest t1ID new, gob_t), (t2ID, origin t2ID new, dest t2ID new, gob_t)])
    )"
 
 definition gung_ho_aux :: "transition \<Rightarrow> transition \<Rightarrow> transition option" where
@@ -629,7 +629,7 @@ fun gung_ho :: update_modifier where
      case gung_ho_aux t1 t2 of
        None \<Rightarrow> None |
        Some gob_t \<Rightarrow> 
-      Some (replace (drop_transitions new {|t2ID|}) t1ID gob_t)
+           Some (replace_transitions new [(t1ID, origin t1ID new, dest t1ID new, gob_t), (t2ID, origin t2ID new, dest t2ID new, gob_t)])
    )"
 
 lemma guard_subset_eq_outputs_updates_subsumption:
